proof/Uniform_distr_proof_ct.ec
@@ -5,8 +5,7 @@ require import JModel List Int AllCore.
 require import Array1.
 require import WArray1.
 
-require import Uniform_distr_extract_ct.
-
+(* SUBTRACTION LEAKAGES  *)
 op sub_prefix : leakages_t = 
   [LeakFor (1, 32); LeakAddr []; LeakAddr [0]; LeakAddr []; 
     LeakAddr []; LeakAddr [0]; LeakAddr [0]].
@@ -22,9 +21,7 @@ axiom sub_g_comp_2 x : 1 < x => sub_g x = sub_step (x-1) ++ sub_g (x - 1).
 
 op sub_f (x : int) : leakages_t = sub_g x ++ sub_prefix.
 
-
-
-lemma jj start_l :
+lemma bn_subc_leakages start_l :
    hoare [ M(Syscall).bn_subc : M.leakages = start_l ==> M.leakages = sub_f 32 ++ start_l ].
 proof. 
 proc.
@@ -39,12 +36,42 @@ smt().
 qed.
 
 
+(* COPY LEAKAGES  *)
+op copy_prefix : leakages_t = LeakFor (0, 32) :: LeakAddr [] ::[].
+op copy_step (i : int) : leakages_t = LeakAddr [i] :: LeakAddr [] :: LeakAddr [i] :: [].
+
+op copy_g (x : int) : leakages_t.
+axiom copy_g_comp_1 x : 0 <= x  => copy_g x = [].
+axiom copy_g_comp_2 x : 0 < x => copy_g x = copy_step (x-1) ++ copy_g (x - 1).
+
+op copy_f (x : int) : leakages_t = copy_g x ++ copy_prefix.
+
+lemma bn_copy_leakages start_l :
+   hoare [ M(Syscall).bn_copy : M.leakages = start_l ==> M.leakages = copy_f 32 ++ start_l ].
+proof. 
+proc.
+sp.  elim*. progress.
+conseq (_: M.leakages = copy_prefix ++ start_l /\ i = 0 ==> _).
+progress.
+while (0 <= i /\ i <= 32 /\ M.leakages = copy_f i ++ start_l).
+wp.  skip.  progress. 
+simplify. smt(). smt(). rewrite /copy_f. rewrite (copy_g_comp_2 (i{hr} +1)).  smt(). simplify. rewrite /copy_step. simplify. auto.
+skip. progress. rewrite /copy_f.  rewrite copy_g_comp_1. auto. auto. 
+smt().
+qed.
+
+
+
+
+(* SAMPLING LEAKAGES  *)
 op samp_prefix : leakages_t = 
   LeakCond true :: LeakAddr [] :: LeakAddr [] :: LeakAddr [] :: LeakAddr [] :: 
   LeakAddr [] :: [].
 op samp_g (x : int) : leakages_t.
 op samp_step (i : int) : leakages_t = LeakCond true :: LeakAddr [] :: LeakAddr [] :: LeakAddr [] :: LeakAddr [] :: (
-sub_f 32 ++ LeakAddr [] :: LeakAddr [] :: []).
+sub_f 32 ++
+LeakAddr [] :: (copy_f 32 ++
+                LeakAddr [] :: LeakAddr [] :: [])) .
 
   
 
@@ -52,15 +79,16 @@ axiom samp_g_comp_1 x : 0 <= x  => samp_g x = [].
 axiom samp_g_comp_2 x : 0 < x => samp_g x = samp_step (x-1) ++ samp_g (x - 1).
 
 op samp_suffix : leakages_t = 
- LeakCond false :: LeakAddr [] :: LeakAddr [] :: LeakAddr [] :: LeakAddr [] :: 
-sub_f 32 ++ LeakAddr [] :: LeakAddr [] :: [].
+ LeakCond false :: LeakAddr [] :: LeakAddr [] :: LeakAddr [] :: LeakAddr [] :: (
+sub_f 32 ++
+LeakAddr [] :: (copy_f 32 ++ LeakAddr [] :: LeakAddr [] :: [])).
 
 op samp_f (x : int) : leakages_t = samp_g x ++ samp_prefix.
 op samp_t (x : int) : leakages_t = samp_suffix ++ samp_f (x - 1).
 
 
 
-lemma ii :
+lemma rsample_leakages :
    hoare [ M(Syscall).rsample : M.leakages = [] ==> M.leakages = samp_t res.`1].
 proc.
 sp. elim*. progress.
@@ -69,10 +97,11 @@ progress.
 while (0 <= i /\ (z = true => M.leakages = samp_f i) 
               /\ (z = false => M.leakages = samp_t i)).
 wp. 
-ecall (jj M.leakages). wp. inline*. wp. rnd. wp.  skip. progress.
+ecall (bn_subc_leakages M.leakages). wp. ecall (bn_copy_leakages M.leakages). wp.  inline*. wp. rnd. wp.  skip. progress.
 smt().  rewrite H4.  rewrite H0. rewrite H2. auto.
 rewrite /samp_f. rewrite (samp_g_comp_2 (i{hr} + 1)). smt().
-simplify. rewrite /samp_step.   
+simplify.
+ rewrite /samp_step.   
 smt(@List). rewrite H4. rewrite H0. rewrite H2. auto.
 rewrite /samp_t. simplify.
 rewrite /samp_suffix. smt(@List).
@@ -82,3 +111,7 @@ rewrite H2. rewrite H. auto.
 auto.
 qed.
     
+
+ (* show that M(syscall) ~ CSpec
+
+  *)
