proof/Ring_ops_proof_ct.ec
@@ -1,8 +1,13 @@
 require import Ring_ops_extract_ct.
 require import JModel List Int AllCore.
 
+
+
 equiv expm_ct :
-  M.expm ~ M.expm :
+  M(Syscall).expm ~ M(Syscall).expm :
   ={M.leakages, glob M} ==> ={M.leakages}.
-proof. proc; inline *; sim. qed.
+proof. 
+
+    proc; inline *; sim. qed.
+
 
